# Assignment 2

## Introduction

In this assignment non-dispersive wave propagation and reflection/transmission of waves in a foundation pile, which is modelled as a bar (Figure 1), are considered. The theory was discussed in Lecture Topic 3 (model for the bar) and in Lecture Topic 8 (non-dispersive waves in an open channel).

### CHANGE Figure HERE
```{figure} ../figures/Assignment_3/A3_Fig1.png
---
width: 100%
name: A1_Fig1
align: center
---
Figure1
```

The 1-D wave equation describes the wave propagation in the bar:
$\rho A \frac{\partial^2 u_x}{\partial t^2} - EA \frac{\partial^2 u_x}{\partial x^2} = 0$

Here, $\rho$, $E$, $A$ denotes the mass density, the Young's modulus and the cross-sectional area of the pile, respectively while $u_x$ denotes the longitudinal displacement.

## Question 1
<iframe src="https://tudelft.h5p.com/content/1292338707597618417/embed" aria-label="Assignment 2 Q1" width="1088" height="1500" frameborder="0" allowfullscreen="allowfullscreen" allow="autoplay *; geolocation *; microphone *; camera *; midi *; encrypted-media *"></iframe><script src="https://tudelft.h5p.com/js/h5p-resizer.js" charset="UTF-8"></script>
<script src="https://tudelft.h5p.com/js/h5p-resizer.js" charset="UTF-8"></script>

````{admonition} Model answer
:class: dropdown

Since for the bar the double plane stress assumption was made (this is always the case if we have a bar), the stresses on the y face (as well as on the z face) are zero. Hence, answer "zero" is the correct one.
````

## Question 2

<iframe src="https://tudelft.h5p.com/content/1292338720762776127/embed" aria-label="Assignment 2 Q2" width="1088" height="637" frameborder="0" allowfullscreen="allowfullscreen" allow="autoplay *; geolocation *; microphone *; camera *; midi *; encrypted-media *"></iframe><script src="https://tudelft.h5p.com/js/h5p-resizer.js" charset="UTF-8"></script>

````{admonition} Model answer
:class: dropdown
We use the plane stress constitutive equations from Topic 3, so

$$\begin{bmatrix}
        \varepsilon_{xx}\\
        \varepsilon_{zz}\\
        \varepsilon_{zx}
    \end{bmatrix}
    =\frac{1}{E}
    \begin{bmatrix}
        1       &-\nu   &0      \\
        -\nu    &1      &0      \\
        0       &0      &1+\nu  
    \end{bmatrix}
    \begin{bmatrix}
        \sigma_{xx}\\
        \sigma_{zz}\\
        \sigma_{zx}
    \end{bmatrix}\\$$ (2.1)

Because of the double plane stress assumption, there is only uni-axial stress, so only axially loaded. Therefore, $\sigma_{zz} = 0$

For the longitudinal strain in $z$ direction we can therefore write

$$\varepsilon_{zz} = -\frac{\nu}{E}\sigma_{xx}$$ (2.2)

Clearly, due the Poisson’s effect, the strains in out of plane directions are non-zero.

Eq.{eq}`2.2` is the sought-for answer.
````

## Question 3

<iframe src="https://tudelft.h5p.com/content/1292338724546617697/embed" aria-label="Assignment 2 Q3" width="1088" height="637" frameborder="0" allowfullscreen="allowfullscreen" allow="autoplay *; geolocation *; microphone *; camera *; midi *; encrypted-media *"></iframe><script src="https://tudelft.h5p.com/js/h5p-resizer.js" charset="UTF-8"></script>

````{admonition} Model answer
:class: dropdown
Look at and keep in mind that:

$$\begin{bmatrix}
        \varepsilon_{xx}\\
        \varepsilon_{zz}\\
        \varepsilon_{zx}
    \end{bmatrix}
    =\frac{1}{E}
    \begin{bmatrix}
        1       &-\nu   &0      \\
        -\nu    &1      &0      \\
        0       &0      &1+\nu  
    \end{bmatrix}
    \begin{bmatrix}
        \sigma_{xx}\\
        \sigma_{zz}\\
        \sigma_{zx}
    \end{bmatrix}\\$$

​
$\sigma_{xx} = E\varepsilon_{xx}$  expresses the correct stress-strain relation for the case of double plane stress (“uni-axial stress”). 

​$\sigma_{xx} = \frac{E}{1- \nu^2} \varepsilon_{xx}$ would be the right stress-strain relation for the case of plane stress and plain strain combined (i.e., for the diaphragm wall; see Lecture 3)

​$\sigma_{xx} = \frac{(1-\nu) E}{(1+\nu)(1- 2\nu)} \varepsilon_{xx}$ would be the right stress-strain relation for the case of double plain strain (“uni-axial strain”; see Assignment 1).
````

## Solution to the 1-D problem of a Semi-infinite bar
We consider the semi-infinite rod shown in Figure 1, which has free end at $x=0$
The transient excitation (hammer blow) is represented in the following simplified manner:

$$ F(t) = F_0, \quad 0<t<t_0$$

$$ F(t) = 0, \quad t>t_0$$

where $t_0 = \frac{L}{4c}$ (i.e., the duration of the pulse is one quarter of the time it takes for a wave to propagate through the entire bar). We assume that the bar is initially at rest.

The general solution of Eq. 1 can be written as follows (D’Alembert’s solution):

$$u_x = u_x^+ \left(t - \frac{x}{c}\right) + u_x \left(t + \frac{x}{c}\right)$$

where, $u_x^+$ denotes a wave propagating in positive direction, and $u_x^-$ in negative direction. Note that we are using the arguments $t - \frac{x}{c}$ and $t + \frac{x}{c}$ instead of $x+ct$ and $x-ct$, respectively (see also Topic 8). This is convenient when dealing with non-homogeneous boundary conditions.


## Question 4

<iframe src="https://tudelft.h5p.com/content/1292338731427623247/embed" aria-label="Assignment 2 Q4" width="1088" height="637" frameborder="0" allowfullscreen="allowfullscreen" allow="autoplay *; geolocation *; microphone *; camera *; midi *; encrypted-media *"></iframe><script src="https://tudelft.h5p.com/js/h5p-resizer.js" charset="UTF-8"></script>

````{admonition} Model answer
:class: dropdown
The expression for $c$ can be determined by substituting the solution (Eq.(5)) into the equation of motion (Eq.(1)). We only demonstrate this for $u_x^+$ (for $u_x^-$ the same result is obtained in the same manner; it is allowed to do handle the solutions separately as Eq.(1) is linear and the superposition principle thus applies).

To determine the temporal and spatial derivatives of $u_x^+$, we first define $\tau = t - \frac{x}{c}$. Then, 

$$\begin{align}
        &\frac{\partial u_x^+}{\partial t} = \frac{\partial u_x^+}{\partial \tau} \frac{\partial \tau}{\partial t} = \frac{\partial u_x^+}{\partial \tau} \cdot 1 \quad &\rightarrow \quad \frac{\partial^2 u_x^+}{\partial t^2} = \frac{\partial^2 u_x^+}{\partial \tau^2} \\
        &\frac{\partial u_x^+}{\partial x} = \frac{\partial u_x^+}{\partial \tau} \frac{\partial \tau}{\partial x} = \frac{\partial u_x^+}{\partial \tau} \cdot \left(-\frac{1}{c}\right) \quad &\rightarrow \quad \frac{\partial^2 u_x^+}{\partial x^2} = \frac{\partial}{\partial x} \left(\frac{\partial u_x^+}{\partial x}\right) =  \frac{\partial}{\partial x} \left( \frac{\partial u_x^+}{\partial \tau} \cdot \left(-\frac{1}{c}\right) \right) = \frac{\partial}{\partial \tau} \left( \frac{\partial u_x^+}{\partial \tau} \cdot \left(-\frac{1}{c}\right) \right) \cdot \frac{\partial \tau}{\partial x} = \frac{\partial^2 u_x^+}{\partial \tau^2} \cdot \left(-\frac{1}{c}\right) \cdot \left(-\frac{1}{c}\right) = \frac{1}{c^2} \frac{\partial^2 u_x^+}{\partial \tau^2}  \\
\end{align}$$

By substituting these derivatives into Eq.(1), we find

$$
\rho A  \frac{\partial^2 u_x^+}{\partial \tau^2} - \frac{EA}{c^2}  \frac{\partial^2 u_x^+}{\partial \tau^2} = \left(\rho A  - \frac{EA}{c^2}\right)  \frac{\partial^2 u_x^+}{\partial \tau^2}  = 0
$$

This equation is satisfied provided that,

$$\begin{align}
c^2 = \frac{E}{\rho} \quad \rightarrow \quad c = \sqrt{\frac{E}{\rho}} > 0
\end{align}$$

Eq.(8) is the sought-for answer.
````

## Question 5

<iframe src="https://tudelft.h5p.com/content/1292338738218068917/embed" aria-label="Assignment 2 Q5" width="1088" height="637" frameborder="0" allowfullscreen="allowfullscreen" allow="autoplay *; geolocation *; microphone *; camera *; midi *; encrypted-media *"></iframe><script src="https://tudelft.h5p.com/js/h5p-resizer.js" charset="UTF-8"></script>

````{admonition} Model answer
:class: dropdown
Starting from the relation between normal force and strain (i.e., the constitutive equation), we can determine the relation between $u_x^+\left(t-\frac{x}{c}\right)$ and $N^+\left(t-\frac{x}{c}\right)$:

$$
N = EA \varepsilon_{xx} \quad \rightarrow \quad N^+\left(t - \frac{x}{c}\right) = EA\frac{\partial}{\partial x} u_x^+\left(t - \frac{x}{c}\right)
$$ (5.1)

Next, we use the fact that $u_x^+\left(t - \frac{x}{c}\right)$ is constant when $t - \frac{x}{c} = \mathrm{constant}$, that is, along

$$
x = ct + \mathrm{constant}
$$ (5.2)

If $u_x^+\left(t - \frac{x}{c}\right) = \mathrm{constant})$ along this line in the $x$, $t$ domain, it implies that its total time derivative is zero:

$$
\frac{du_x^+}{dt} = \frac{\partial u_x^+}{\partial t} + \frac{\partial u_x^+}{\partial x}\frac{\partial x}{\partial t} = 0 \quad \rightarrow \quad \frac{\partial u_x^+}{\partial x} = -\frac{1}{c} \frac{\partial u_x^+}{\partial t}
$$ (5.3)

In the last step, the time derivative of Eq.{eq}`5.2` was used.

Now, Eqs.{eq}`5.1` and {eq}`5.3` can be combined to obtain

$$
N^+ = -\frac{EA}{c}\frac{\partial u_x^+}{\partial t} = - \frac{EA}{c} v_x^+ \quad \rightarrow \quad v_x^+\left(t - \frac{x}{c}\right) = -\frac{c}{EA} N^+\left(t - \frac{x}{c}\right)
$$ (5.4)

Eq.{eq}`5.4` (the last expression) is the sought-for answer.
````

## Question 6

<iframe src="https://tudelft.h5p.com/content/1292339560346587247/embed" aria-label="Assignment 2 Q6" width="1088" height="637" frameborder="0" allowfullscreen="allowfullscreen" allow="autoplay *; geolocation *; microphone *; camera *; midi *; encrypted-media *"></iframe><script src="https://tudelft.h5p.com/js/h5p-resizer.js" charset="UTF-8"></script>

````{admonition} Model answer
:class: dropdown
Starting from the relation between normal force and strain (i.e., the constitutive equation), we can determine the relation between $u_x^-\left(t+\frac{x}{c}\right)$ and $N^-\left(t+\frac{x}{c}\right)$:

$$
N = EA \varepsilon_{xx} \quad \rightarrow \quad N^+\left(t - \frac{x}{c}\right) = EA\frac{\partial}{\partial x} u_x^+\left(t - \frac{x}{c}\right)
$$ (6.1)

Next, we use the fact that $u_x^-\left(t + \frac{x}{c}\right)$ is constant when $t + \frac{x}{c} = \mathrm{constant}$, that is, along

$$
x = -ct + \mathrm{constant}
$$ (6.2)

If $u_x^-\left(t + \frac{x}{c}\right) = \mathrm{constant})$ along this line in the $x$, $t$ domain, it implies that its total time derivative is zero:

$$
\frac{du_x^-}{dt} = \frac{\partial u_x^-}{\partial t} + \frac{\partial u_x^-}{\partial x}\frac{\partial x}{\partial t} = 0 \quad \rightarrow \quad \frac{\partial u_x^-}{\partial x} = +\frac{1}{c} \frac{\partial u_x^-}{\partial t}
$$ (6.3)

In the last step, the time derivative of Eq.{eq}`6.2` was used.

Now, Eqs.{eq}`6.1` and {eq}`6.3` can be combined to obtain

$$
N^- = +\frac{EA}{c}\frac{\partial u_x^-}{\partial t} = \frac{EA}{c} v_x^- \quad \rightarrow \quad v_x^-\left(t + \frac{x}{c}\right) = +\frac{c}{EA} N^-\left(t + \frac{x}{c}\right)
$$ (6.4)

Eq.{eq}`6.4` (the last expression) is the sought-for answer.
````


## Question 7

<iframe src="https://tudelft.h5p.com/content/1292339567866245247/embed" aria-label="Assignment 2 Q7" width="1088" height="637" frameborder="0" allowfullscreen="allowfullscreen" allow="autoplay *; geolocation *; microphone *; camera *; midi *; encrypted-media *"></iframe><script src="https://tudelft.h5p.com/js/h5p-resizer.js" charset="UTF-8"></script><script src="https://tudelft.h5p.com/js/h5p-resizer.js" charset="UTF-8"></script>

(NO MODAL ANSWER)

## Question 8

<iframe src="https://tudelft.h5p.com/content/1292339569127728047/embed" aria-label="Assignment 2 Q8" width="1088" height="637" frameborder="0" allowfullscreen="allowfullscreen" allow="autoplay *; geolocation *; microphone *; camera *; midi *; encrypted-media *"></iframe><script src="https://tudelft.h5p.com/js/h5p-resizer.js" charset="UTF-8"></script>

````{admonition} Model answer
:class: dropdown
To answer this question, we need to determine the reflected wave based on the boundary coniditon at the free end. It reads

$$
N(x = L, t) = 0
$$ (7.1)

The Method of the Images can be employed to determine the reflected wave. It will be applied in terms of normal force and particle velocity as these quantities are one to one related (see Eqs. {eq}`6.4` and Eqs. {eq}`6.4`). The Method of the Images is schematically illustraed in the figure below. The starting point is that a compression wave (as stated in the question; we assume for now an arbitrary shape and will determine the precise shape in the next question) propagates through the bar, as shown in the bottom left. Then, in order to respect the boundary condition (Eq. {eq}`7.1` at $x = L$, the normal force associated with the image wave (which will be the reflected wave as soon as it enters the real domain) will have to have the same shape but opposite sign. Thus, the normal force changes sign during reflection. Hence, a compressional wave is reflected as a tensile wave (and vice versa). Thus the correct answer for the question is Tensile Wave.

Even though not asked, for completeness we note that the particle velocities corresponding with the incident and reflected waves can be determined using Eqs. 
 {eq}`6.4` and Eqs. {eq}`6.4`. Clearly, the particle-velocity pulses have the same shape and also the same sign; see also question 10.

(ADD FIGURE HERE) 
````

## Question 9

<iframe src="https://tudelft.h5p.com/content/1292339573139943837/embed" aria-label="Assignment 2 Q9" width="1088" height="637" frameborder="0" allowfullscreen="allowfullscreen" allow="autoplay *; geolocation *; microphone *; camera *; midi *; encrypted-media *"></iframe><script src="https://tudelft.h5p.com/js/h5p-resizer.js" charset="UTF-8"></script>

````{admonition} Model answer
:class: dropdown
We determine the rightward propagating wave based on the boundary condition at $x = 0$ (Eq.{eq}``6.4``). Using Eq.{eq}`5.2`, we can write (assuming zero initial velocity)

$$
v_x^+(t) = -\frac{c}{EA} N^+(t) = \frac{c}{EA}
\begin{align}
\begin{cases}
0, \quad {\raggedleft t<0}&\\
F_0, \quad {\raggedleft 0<t<t_0}&\\
0, \quad {\raggedleft t>t_0}&
\end{cases}
\end{align}
$$ (9.1)

With the known time signature of the particle velocity (Eq.{eq}`9.1`), the rightward propagating wave is essentially known throughout the entire bar as the wave is non-dispersive. Therefore, by introducing the following replacement, $t \rightarrow t - \frac{x}{c}$, we obtain

$$
v_x^+\left(t - \frac{x}{c}\right) = \frac{c}{EA}
\begin{align}
\begin{cases}
0, \quad \rightline{ t - \frac{x}{c}<0}&\\
F_0, \quad \rightline{ 0<t - \frac{x}{c}<t_0}&\\
0, \quad \rightline{ t - \frac{x}{c}>t_0}&
\end{cases}
\end{align}
$$ (9.2)

To visualize the particle-velocity field spatially (ad in view of the application of the Method of the Images to determine the reflected wave; see later), we slightly rewrite this result:

$$
v_x^+\left(t - \frac{x}{c}\right) = \frac{c}{EA}
\begin{cases}
\lreqn{0}{x>ct}\\
\lreqn{F_0}{c(t - t_0) < x < ct}\\
\lreqn{0}{x<c(t - t_0)}
\end{cases}
$$ (9.3)

LR EQN USED HERE

Eq.{eq}`9.3` is the sought-for answer. The result in graphically represented in the figure below. Indeed the rightward propagating wave is a compression wave, as is clear from the corresponding normal force being negative. (Note that we have now derived this, while in the previous question we assumed the incident wave to be a compressional one)

(ADD FIGURE HERE)

Note that Eqs{eq}`9.2` and {eq}`9.3` are only valid for $0<t<\frac{2L}{c}$. Beyond $t = \frac{2L}{c}$ (the moment that the wave reflected from $x = L$ has reached $x = 0$), a different expression for the rightward propagating wave would need to be found.
````


## Question 10

<iframe src="https://tudelft.h5p.com/content/1292339584547771737/embed" aria-label="Assignment 2 Q10" width="1088" height="637" frameborder="0" allowfullscreen="allowfullscreen" allow="autoplay *; geolocation *; microphone *; camera *; midi *; encrypted-media *"></iframe><script src="https://tudelft.h5p.com/js/h5p-resizer.js" charset="UTF-8"></script>

````{admonition} Model answer
:class: dropdown
The figure related to question 9 illustrates the rightward propagating wave as well as the image/reflected wave for the specific excitation. Using $v_x(x = L, t) = v_x^+(x = L, t) + v_x^-(x = L, t)$ and the fact that v_x^-(x = L, t) = v_x^+(x = L, t)$, we find that the total particle velocity at the right end is doubled during reflection:

$$
v_x(x = L, t)\bigg|_{max} = 2 \frac{F_0 c}{EA}
$$ (10.1)

Eq.{eq}`10.1` is the sought-for answer.

We could have formulated an expression for the reflected wave (which originates from the image boundary $x = 2L$), but that is not really necessary for the required answer.
````

## Question 11

<iframe src="https://tudelft.h5p.com/content/1292339588915708467/embed" aria-label="Assignment 2 Q11" width="1088" height="637" frameborder="0" allowfullscreen="allowfullscreen" allow="autoplay *; geolocation *; microphone *; camera *; midi *; encrypted-media *"></iframe><script src="https://tudelft.h5p.com/js/h5p-resizer.js" charset="UTF-8"></script>

## Question 12

<iframe src="https://tudelft.h5p.com/content/1292339590864887557/embed" aria-label="Assignment 2 Q12" width="1088" height="637" frameborder="0" allowfullscreen="allowfullscreen" allow="autoplay *; geolocation *; microphone *; camera *; midi *; encrypted-media *"></iframe><script src="https://tudelft.h5p.com/js/h5p-resizer.js" charset="UTF-8"></script>


## Question 13

<iframe src="https://tudelft.h5p.com/content/1292339594296058477/embed" aria-label="Assignment 2 Q13" width="1088" height="637" frameborder="0" allowfullscreen="allowfullscreen" allow="autoplay *; geolocation *; microphone *; camera *; midi *; encrypted-media *"></iframe><script src="https://tudelft.h5p.com/js/h5p-resizer.js" charset="UTF-8"></script>


## Question 14

<iframe src="https://tudelft.h5p.com/content/1292339774065403397/embed" aria-label="Assignment 2 Q14_1" width="1088" height="637" frameborder="0" allowfullscreen="allowfullscreen" allow="autoplay *; geolocation *; microphone *; camera *; midi *; encrypted-media *"></iframe><script src="https://tudelft.h5p.com/js/h5p-resizer.js" charset="UTF-8"></script>


## Question 15

<iframe src="https://tudelft.h5p.com/content/1292339779964332597/embed" aria-label="Assignment 2 Q15" width="1088" height="637" frameborder="0" allowfullscreen="allowfullscreen" allow="autoplay *; geolocation *; microphone *; camera *; midi *; encrypted-media *"></iframe><script src="https://tudelft.h5p.com/js/h5p-resizer.js" charset="UTF-8"></script>


## Question 16

<iframe src="https://tudelft.h5p.com/content/1292339784471130187/embed" aria-label="Assignment 2 Q16" width="1088" height="637" frameborder="0" allowfullscreen="allowfullscreen" allow="autoplay *; geolocation *; microphone *; camera *; midi *; encrypted-media *"></iframe><script src="https://tudelft.h5p.com/js/h5p-resizer.js" charset="UTF-8"></script>





